---
comments: true
difficulty: Easy
edit_url: https://github.com/doocs/leetcode/edit/main/solution/1800-1899/1880.Check%20if%20Word%20Equals%20Summation%20of%20Two%20Words/README_EN.md
rating: 1187
source: Weekly Contest 243 Q1
tags:
    - String
---

<!-- problem:start -->

# [1880. Check if Word Equals Summation of Two Words](https://leetcode.com/problems/check-if-word-equals-summation-of-two-words)

[中文文档](/solution/1800-1899/1880.Check%20if%20Word%20Equals%20Summation%20of%20Two%20Words/README.md)

## Description

<!-- description:start -->

<p>The <strong>letter value</strong> of a letter is its position in the alphabet <strong>starting from 0</strong> (i.e. <code>&#39;a&#39; -&gt; 0</code>, <code>&#39;b&#39; -&gt; 1</code>, <code>&#39;c&#39; -&gt; 2</code>, etc.).</p>

<p>The <strong>numerical value</strong> of some string of lowercase English letters <code>s</code> is the <strong>concatenation</strong> of the <strong>letter values</strong> of each letter in <code>s</code>, which is then <strong>converted</strong> into an integer.</p>

<ul>
	<li>For example, if <code>s = &quot;acb&quot;</code>, we concatenate each letter&#39;s letter value, resulting in <code>&quot;021&quot;</code>. After converting it, we get <code>21</code>.</li>
</ul>

<p>You are given three strings <code>firstWord</code>, <code>secondWord</code>, and <code>targetWord</code>, each consisting of lowercase English letters <code>&#39;a&#39;</code> through <code>&#39;j&#39;</code> <strong>inclusive</strong>.</p>

<p>Return <code>true</code> <em>if the <strong>summation</strong> of the <strong>numerical values</strong> of </em><code>firstWord</code><em> and </em><code>secondWord</code><em> equals the <strong>numerical value</strong> of </em><code>targetWord</code><em>, or </em><code>false</code><em> otherwise.</em></p>

<p>&nbsp;</p>
<p><strong class="example">Example 1:</strong></p>

<pre>
<strong>Input:</strong> firstWord = &quot;acb&quot;, secondWord = &quot;cba&quot;, targetWord = &quot;cdb&quot;
<strong>Output:</strong> true
<strong>Explanation:</strong>
The numerical value of firstWord is &quot;acb&quot; -&gt; &quot;021&quot; -&gt; 21.
The numerical value of secondWord is &quot;cba&quot; -&gt; &quot;210&quot; -&gt; 210.
The numerical value of targetWord is &quot;cdb&quot; -&gt; &quot;231&quot; -&gt; 231.
We return true because 21 + 210 == 231.
</pre>

<p><strong class="example">Example 2:</strong></p>

<pre>
<strong>Input:</strong> firstWord = &quot;aaa&quot;, secondWord = &quot;a&quot;, targetWord = &quot;aab&quot;
<strong>Output:</strong> false
<strong>Explanation:</strong> 
The numerical value of firstWord is &quot;aaa&quot; -&gt; &quot;000&quot; -&gt; 0.
The numerical value of secondWord is &quot;a&quot; -&gt; &quot;0&quot; -&gt; 0.
The numerical value of targetWord is &quot;aab&quot; -&gt; &quot;001&quot; -&gt; 1.
We return false because 0 + 0 != 1.
</pre>

<p><strong class="example">Example 3:</strong></p>

<pre>
<strong>Input:</strong> firstWord = &quot;aaa&quot;, secondWord = &quot;a&quot;, targetWord = &quot;aaaa&quot;
<strong>Output:</strong> true
<strong>Explanation:</strong> 
The numerical value of firstWord is &quot;aaa&quot; -&gt; &quot;000&quot; -&gt; 0.
The numerical value of secondWord is &quot;a&quot; -&gt; &quot;0&quot; -&gt; 0.
The numerical value of targetWord is &quot;aaaa&quot; -&gt; &quot;0000&quot; -&gt; 0.
We return true because 0 + 0 == 0.
</pre>

<p>&nbsp;</p>
<p><strong>Constraints:</strong></p>

<ul>
	<li><code>1 &lt;= firstWord.length, </code><code>secondWord.length, </code><code>targetWord.length &lt;= 8</code></li>
	<li><code>firstWord</code>, <code>secondWord</code>, and <code>targetWord</code> consist of lowercase English letters from <code>&#39;a&#39;</code> to <code>&#39;j&#39;</code> <strong>inclusive</strong>.</li>
</ul>

<!-- description:end -->

## Solutions

<!-- solution:start -->

### Solution 1

<!-- tabs:start -->

#### Python3

```python
class Solution:
    def isSumEqual(self, firstWord: str, secondWord: str, targetWord: str) -> bool:
        def f(s):
            res = 0
            for c in s:
                res = res * 10 + (ord(c) - ord('a'))
            return res

        return f(firstWord) + f(secondWord) == f(targetWord)
```

#### Java

```java
class Solution {
    public boolean isSumEqual(String firstWord, String secondWord, String targetWord) {
        return f(firstWord) + f(secondWord) == f(targetWord);
    }

    private int f(String s) {
        int res = 0;
        for (char c : s.toCharArray()) {
            res = res * 10 + (c - 'a');
        }
        return res;
    }
}
```

#### C++

```cpp
class Solution {
public:
    bool isSumEqual(string firstWord, string secondWord, string targetWord) {
        return f(firstWord) + f(secondWord) == f(targetWord);
    }

    int f(string s) {
        int res = 0;
        for (char c : s) res = res * 10 + (c - 'a');
        return res;
    }
};
```

#### Go

```go
func isSumEqual(firstWord string, secondWord string, targetWord string) bool {
	f := func(s string) int {
		res := 0
		for _, c := range s {
			res = res*10 + int(c-'a')
		}
		return res
	}
	return f(firstWord)+f(secondWord) == f(targetWord)
}
```

#### TypeScript

```ts
function isSumEqual(firstWord: string, secondWord: string, targetWord: string): boolean {
    const calc = (s: string) => {
        let res = 0;
        for (const c of s) {
            res = res * 10 + c.charCodeAt(0) - 'a'.charCodeAt(0);
        }
        return res;
    };
    return calc(firstWord) + calc(secondWord) === calc(targetWord);
}
```

#### Rust

```rust
impl Solution {
    fn calc(s: &String) -> i32 {
        let mut res = 0;
        for c in s.as_bytes() {
            res = res * 10 + ((c - b'a') as i32);
        }
        res
    }

    pub fn is_sum_equal(first_word: String, second_word: String, target_word: String) -> bool {
        Self::calc(&first_word) + Self::calc(&second_word) == Self::calc(&target_word)
    }
}
```

#### JavaScript

```js
/**
 * @param {string} firstWord
 * @param {string} secondWord
 * @param {string} targetWord
 * @return {boolean}
 */
var isSumEqual = function (firstWord, secondWord, targetWord) {
    function f(s) {
        let res = 0;
        for (let c of s) {
            res = res * 10 + (c.charCodeAt() - 'a'.charCodeAt());
        }
        return res;
    }
    return f(firstWord) + f(secondWord) == f(targetWord);
};
```

#### C

```c
int calc(char* s) {
    int res = 0;
    for (int i = 0; s[i]; i++) {
        res = res * 10 + s[i] - 'a';
    }
    return res;
}

bool isSumEqual(char* firstWord, char* secondWord, char* targetWord) {
    return calc(firstWord) + calc(secondWord) == calc(targetWord);
}
```

<!-- tabs:end -->

<!-- solution:end -->

<!-- problem:end -->
